name changes && start of Challenge Prob 4

Source/NIP_LLVM/NIP_LLVMMain.cs
@@ -1,0 +1,60 @@
+using System;
+using System.IO;
+using System.Collections.Generic;
+using System.Diagnostics.Contracts;
+using System.Reflection;
+namespace NIP.LLVM
+{
+    public class IllegalDafnyFile : Exception { }
+    
+    public class DafnyFile {
+    public string FilePath { get; private set; }
+    public string BaseName { get; private set; }
+    public bool isPrecompiled { get; private set; }
+    public string SourceFileName { get; private set; }
+
+    public static List<string> fileNames(IList<DafnyFile> dafnyFiles) {
+      var sourceFiles = new List<string>();
+      foreach (DafnyFile f in dafnyFiles) {
+        sourceFiles.Add(f.FilePath);
+      }
+      return sourceFiles;
+    }
+
+    // public DafnyFile(string filePath) {
+    //   FilePath = filePath;
+    //   BaseName = Path.GetFileName(filePath);
+
+    //   var extension = Path.GetExtension(filePath);
+    //   if (extension != null) { extension = extension.ToLower(); }
+
+    //   if (extension == ".dfy" || extension == ".dfyi" || extension == ".cdfy" || extension == ".arm") {
+    //     isPrecompiled = false;
+    //     SourceFileName = filePath;
+    //   } else if (extension == ".dll") {
+    //     isPrecompiled = true;
+    //     Assembly.ReflectionOnlyLoad("DafnyRuntime");
+    //     var asm = Assembly.ReflectionOnlyLoadFrom(filePath);
+    //     string sourceText = null;
+    //     foreach (var adata in asm.GetCustomAttributesData()) {
+    //       if (adata.Constructor.DeclaringType.Name == "DafnySourceAttribute") {
+    //         foreach (var args in adata.ConstructorArguments) {
+    //           if (args.ArgumentType == System.Type.GetType("System.String")) {
+    //             sourceText = (string)args.Value;
+    //           }
+    //         }
+    //       }
+    //     }
+
+    //     if (sourceText == null) { throw new IllegalDafnyFile(); }
+    //     SourceFileName = Path.GetTempFileName();
+    //     File.WriteAllText(SourceFileName, sourceText);
+
+    //   } else {
+    //     throw new IllegalDafnyFile();
+    //   }
+
+
+    // }
+  }
+}
