Dafny/examples/Challenge4.i.dfy
@@ -1,0 +1,98 @@
+include "../LLVM/llvm.i.dfy"
+include "../LLVM/control_flow.i.dfy"
+include "../LLVM/generalInstructions.i.dfy"
+include "../LLVM/types.dfy"
+include "../LLVM/memory.i.dfy"
+include "../LLVM/Operations/otherOperations.i.dfy"
+
+
+module musings {
+    import opened LLVM_def
+    import opened control_flow
+    import opened general_instructions
+    import opened types
+    import opened memory
+    import opened other_operations_i
+
+
+// VULN
+// ; Function Attrs: nofree nosync nounwind uwtable
+// define dso_local void @choose_new_sa(i32 %current_index, i32 %iterations, i32* nocapture %avail_addrs) local_unnamed_addr #12 {
+// entry:
+//   %cmp17 = icmp sgt i32 %iterations, 255
+//   br i1 %cmp17, label %if.then, label %if.end
+
+// if.then:                                          ; preds = %if.end5, %entry
+//   store i8 -2, i8* getelementptr inbounds (%struct.conf_t, %struct.conf_t* @conf, i64 0, i32 3), align 8, !tbaa !20
+//   br label %return
+
+// if.end:                                           ; preds = %entry, %if.end5
+//   %iterations.tr19 = phi i32 [ %inc6, %if.end5 ], [ %iterations, %entry ]
+//   %current_index.tr18 = phi i32 [ %rem, %if.end5 ], [ %current_index, %entry ]
+//   %idxprom = sext i32 %current_index.tr18 to i64
+//   %arrayidx = getelementptr inbounds i32, i32* %avail_addrs, i64 %idxprom
+//   %0 = load i32, i32* %arrayidx, align 4, !tbaa !13
+//   %cmp1 = icmp eq i32 %0, 1
+//   br i1 %cmp1, label %if.then2, label %if.end5
+
+// if.then2:                                         ; preds = %if.end
+//   %arrayidx.le = getelementptr inbounds i32, i32* %avail_addrs, i64 %idxprom
+//   %conv = trunc i32 %current_index.tr18 to i8
+//   store i8 %conv, i8* getelementptr inbounds (%struct.conf_t, %struct.conf_t* @conf, i64 0, i32 3), align 8, !tbaa !20
+//   store i32 0, i32* %arrayidx.le, align 4, !tbaa !13
+//   br label %return
+
+// if.end5:                                          ; preds = %if.end
+//   %inc = add nsw i32 %current_index.tr18, 1
+//   %inc6 = add i32 %iterations.tr19, 1
+//   %rem = srem i32 %inc, 254
+//   %exitcond = icmp eq i32 %inc6, 256
+//   br i1 %exitcond, label %if.then, label %if.end
+
+// return:                                           ; preds = %if.then2, %if.then
+//   ret void
+// }
+
+/// -------------------------------------------
+//  Simplified.... 
+/// -------------------------------------------
+
+
+// define dso_local void @choose_new_sa(i32 %current_index, i32 %iterations, i32* nocapture %avail_addrs) local_unnamed_addr #12 {
+// entry:
+//   %cmp17 = icmp sgt i32 %iterations, 255
+//   br i1 %cmp17, label %if.then, label %return
+
+// if.then:                                          ; preds = %if.end5, %entry
+//   store i8 -2, i8* getelementptr inbounds (%struct.conf_t, %struct.conf_t* @conf, i64 0, i32 3), align 8, !tbaa !20
+//   br label %return
+
+// return:                                           ; preds = %if.then2, %if.then
+//   ret void
+// }
+
+
+function {:opaque} demo_challenge_prob_4(s:MemState,current_index:lvm_operand_opr,
+                                         iterations:lvm_operand_opr,avail_addrs:lvm_operand_opr,cmp17:lvm_operand_opr):lvm_code
+{
+    reveal_IntFits();
+    var remaining := D(Int(255,IntType(4,false)));
+    var current_sa := D(Ptr(0,0,0));
+ 
+    var returnLabel:code := lvm_Block(lvm_Codes(Ins(RET(D(Void))),lvm_CNil()));         // return: 
+                                                                                        //   ret void
+    
+    var ifThenLabel:code := lvm_Block(lvm_Codes(Ins(STORE(D(Int(2,IntType(1,false))),current_sa,s)),  //   store i8 -2, i8* getelementptr inbounds (%struct.conf_t, %struct.conf_t* @conf, i64 0, i32 3), align 8, !tbaa !20
+                                       lvm_Codes(Ins(UNCONDBR(returnLabel.block)),lvm_CNil())));      //   br label %return
+                                                                                                             
+      
+    lvm_Block(lvm_Codes(Ins(ICMP(cmp17,sgt,4,iterations,remaining)),             // %cmp17 = icmp sgt i32 %iterations, 255
+              lvm_Codes(Ins(BR(cmp17,                                            // br i1 %cmp17, label %if.then, label %return
+                lvm_Codes(ifThenLabel,lvm_CNil()),
+                lvm_Codes(returnLabel,lvm_CNil()))),  
+              lvm_Codes(Ins(RET(D(Void))),lvm_CNil()))))                           
+
+}
+
+}
+
