Dafny/examples/demoChallengeProb1Vuln.i.dfy
@@ -94,23 +94,23 @@ function {:opaque} demo_challenge_prob_1_code(speed_value:lvm_operand_opr,s:MemS
     var shl_amount := D(Int(8,IntType(2,false)));
 
 
-    lvm_Block(lvm_CCons(Ins(GETELEMENTPTR(var_5,1,var_0,index3)),                         // %5 = getelementptr inbounds i8, i8* %0, i64 3
-              lvm_CCons(Ins(LOAD(var_6,s,1,var_5)),                                       // %6 = load i8, i8* %2, align 1, !tbaa !4
-              lvm_CCons(Ins(ZEXT(var_7,1,var_6,2)),                                       // %7 = zext i8 %3 to i16
-              lvm_CCons(Ins(SHL(var_8,var_7,shl_amount)),                                 // %8 = shl i32 %7, 8
-              lvm_CCons(Ins(GETELEMENTPTR(var_10,1,var_0,index2)),                        // %10 = getelementptr inbounds i8, i8* %0, i64 2
-              lvm_CCons(Ins(LOAD(var_11,s,1,var_10)),                                     // %11 = load i8, i8* %10, align 1
-              lvm_CCons(Ins(ZEXT(var_12,1,var_11,2)),                                     // %12 = zext i8 %11 to i16
-              lvm_CCons(Ins(ADD(speed_value,2,var_8,var_12)),                             // %13 = add nsw i16 %8, %12
-              lvm_CCons(Ins(ICMP(var_17,sgt,2,speed_value,D(Int(0,IntType(2,false))))),   // %17 = icmp sgt i16 %13, 0  <--------
-              lvm_CCons(Ins(RET(D(Void))),lvm_CNil())))))))))))                           // ret void
+    lvm_Block(lvm_Codes(Ins(GETELEMENTPTR(var_5,1,var_0,index3)),                         // %5 = getelementptr inbounds i8, i8* %0, i64 3
+              lvm_Codes(Ins(LOAD(var_6,s,1,var_5)),                                       // %6 = load i8, i8* %2, align 1, !tbaa !4
+              lvm_Codes(Ins(ZEXT(var_7,1,var_6,2)),                                       // %7 = zext i8 %3 to i16
+              lvm_Codes(Ins(SHL(var_8,var_7,shl_amount)),                                 // %8 = shl i32 %7, 8
+              lvm_Codes(Ins(GETELEMENTPTR(var_10,1,var_0,index2)),                        // %10 = getelementptr inbounds i8, i8* %0, i64 2
+              lvm_Codes(Ins(LOAD(var_11,s,1,var_10)),                                     // %11 = load i8, i8* %10, align 1
+              lvm_Codes(Ins(ZEXT(var_12,1,var_11,2)),                                     // %12 = zext i8 %11 to i16
+              lvm_Codes(Ins(ADD(speed_value,2,var_8,var_12)),                             // %13 = add nsw i16 %8, %12
+              lvm_Codes(Ins(ICMP(var_17,sgt,2,speed_value,D(Int(0,IntType(2,false))))),   // %17 = icmp sgt i16 %13, 0  <--------
+              lvm_Codes(Ins(RET(D(Void))),lvm_CNil())))))))))))                           // ret void
 
 }
  
 
 
 
-lemma lvm_demo_simple_challenge_prob_1(lvm_b0:lvm_codes, lvm_s0:lvm_state,var_0:lvm_operand_opr,var_5:lvm_operand_opr,var_6:lvm_operand_opr,var_7:lvm_operand_opr,var_8:lvm_operand_opr,var_10:lvm_operand_opr,var_11:lvm_operand_opr,var_12:lvm_operand_opr,speed_value:lvm_operand_opr, var_17:lvm_operand_opr)
+lemma lvm_demo_simple_challenge_prob_1_vuln(lvm_b0:lvm_codes, lvm_s0:lvm_state,var_0:lvm_operand_opr,var_5:lvm_operand_opr,var_6:lvm_operand_opr,var_7:lvm_operand_opr,var_8:lvm_operand_opr,var_10:lvm_operand_opr,var_11:lvm_operand_opr,var_12:lvm_operand_opr,speed_value:lvm_operand_opr, var_17:lvm_operand_opr)
       returns (lvm_bM:lvm_codes, lvm_sM:lvm_state,lvm_sMs:seq<lvm_state>)
 // PRE Conditions 
 
